IsaSAT: mark new clauses as used

Weidenbach_Book/IsaSAT_Clauses.thy
@@ -472,7 +472,7 @@ than reserving a space that is large enough directly. However, in this case the 
 is so large that there should not be any difference\<close>
 definition fm_add_new where
  \<open>fm_add_new b C N = do {
-    let st = (if b then AStatus IRRED False else AStatus LEARNED False);
+    let st = (if b then AStatus IRRED True else AStatus LEARNED True);
     let l = length N;
     let s = length C - 2;
     let N = (if is_short_clause C then
@@ -529,7 +529,16 @@ lemma AStatus_IRRED [sepref_fr_rules]:
   \<open>(uncurry0 (return 0), uncurry0 (RETURN AStatus_IRRED)) \<in> unit_assn\<^sup>k \<rightarrow>\<^sub>a arena_el_assn\<close>
   by sepref_to_hoare
     (sep_auto simp: AStatus_IRRED_def arena_el_rel_def hr_comp_def uint32_nat_rel_def br_def
-    status_rel_def bitfield_rel_def nat_0_AND)
+      status_rel_def bitfield_rel_def nat_0_AND)
+
+definition AStatus_IRRED2 where
+  \<open>AStatus_IRRED2 = AStatus IRRED True\<close>
+
+lemma AStatus_IRRED2 [sepref_fr_rules]:
+  \<open>(uncurry0 (return 0b100), uncurry0 (RETURN AStatus_IRRED2)) \<in> unit_assn\<^sup>k \<rightarrow>\<^sub>a arena_el_assn\<close>
+  by sepref_to_hoare
+    (sep_auto simp: AStatus_IRRED2_def arena_el_rel_def hr_comp_def uint32_nat_rel_def br_def
+      status_rel_def bitfield_rel_def nat_0_AND)
 
 definition AStatus_LEARNED where
   \<open>AStatus_LEARNED = AStatus LEARNED True\<close>
@@ -538,7 +547,7 @@ lemma AStatus_LEARNED [sepref_fr_rules]:
   \<open>(uncurry0 (return 0b101), uncurry0 (RETURN AStatus_LEARNED)) \<in> unit_assn\<^sup>k \<rightarrow>\<^sub>a arena_el_assn\<close>
   by sepref_to_hoare
     (sep_auto simp: AStatus_LEARNED_def arena_el_rel_def hr_comp_def uint32_nat_rel_def br_def
-    status_rel_def bitfield_rel_def)
+      status_rel_def bitfield_rel_def)
 
 
 definition AStatus_LEARNED2 where
@@ -601,7 +610,7 @@ sepref_definition append_and_length_code
   :: \<open>[\<lambda>((b, C), N). length C \<le> uint32_max+2 \<and> length C \<ge> 2]\<^sub>a bool_assn\<^sup>k *\<^sub>a clause_ll_assn\<^sup>d *\<^sub>a (arena_assn)\<^sup>d \<rightarrow>
        arena_assn *a nat_assn\<close>
   supply [[goals_limit=1]] le_uint32_max_le_uint64_max[intro]
-  unfolding fm_add_new_def AStatus_IRRED_def[symmetric]
+  unfolding fm_add_new_def AStatus_IRRED_def[symmetric] AStatus_IRRED2_def[symmetric]
    AStatus_LEARNED_def[symmetric] AStatus_LEARNED2_def[symmetric]
    two_uint64_nat_def[symmetric]
    apply (rewrite in \<open>let _ = _ - _ in _\<close> length_uint64_nat_def[symmetric])
@@ -677,6 +686,7 @@ sepref_definition (in -)append_and_length_fast_code
     header_size_def[simp]
   unfolding fm_add_new_def AStatus_IRRED_def[symmetric] append_and_length_fast_code_pre_def
    AStatus_LEARNED_def[symmetric] AStatus_LEARNED2_def[symmetric]
+   AStatus_IRRED2_def[symmetric]
    two_uint64_nat_def[symmetric] fm_add_new_fast_def
    apply (rewrite in \<open>let _ = _ - _ in _\<close> length_uint64_nat_def[symmetric])
    apply (rewrite in \<open>let _ = _ in _\<close> length_uint64_nat_def[symmetric])
@@ -689,7 +699,7 @@ declare append_and_length_fast_code.refine[sepref_fr_rules]
 
 lemma fm_add_new_alt_def:
  \<open>fm_add_new b C N = do {
-      let st = (if b then AStatus_IRRED else AStatus_LEARNED2);
+      let st = (if b then AStatus_IRRED2 else AStatus_LEARNED);
       let l = length_uint64_nat N;
       let s = uint32_of_uint64_conv (length_uint64_nat C - two_uint64_nat);
       let N =
@@ -709,7 +719,8 @@ lemma fm_add_new_alt_def:
           (zero_uint64_nat, N);
       RETURN (N, l + header_size C)
     }\<close>
-  unfolding fm_add_new_def Let_def AStatus_LEARNED2_def AStatus_IRRED_def
+  unfolding fm_add_new_def Let_def AStatus_LEARNED2_def AStatus_IRRED2_def
+     AStatus_LEARNED_def AStatus_IRRED_def
   by auto
 
 definition fmap_swap_ll_u64 where
